DenotSem/Denot.thy
@@ -5,9 +5,12 @@ begin
 abbreviation fun_app :: "ty \<Rightarrow> ty \<Rightarrow> ty set" (infix "\<bullet>" 80) where
   "f \<bullet> v \<equiv> {v'. f <: v \<rightarrow> v' \<and> wf_ty v' }"
 
+abbreviation up :: "ty \<Rightarrow> ty set" ("\<up>" 1000) where
+  "up A \<equiv> {B. A <: B \<and> wf_ty B}"
+  
 fun E :: "exp \<Rightarrow> ty list \<Rightarrow> ty set" ("\<lbrakk>_\<rbrakk>_" [999] 1000) where
   Enat: "\<lbrakk>ENat n\<rbrakk> \<rho> = { TNat n }" |
-  Evar: "\<lbrakk>EVar k\<rbrakk> \<rho> = (if k < length \<rho> then {\<rho>!k} else {})" |
+  Evar: "\<lbrakk>EVar k\<rbrakk> \<rho> = (if k < length \<rho> then \<up>(\<rho>!k) else {})" |
   Elam: "\<lbrakk>ELam e\<rbrakk> \<rho> = { f. wf_fun f \<and> (\<forall>v v'. v\<rightarrow>v' \<in> atoms f \<longrightarrow> v' \<in> \<lbrakk>e\<rbrakk>(v#\<rho>)) }" |
   Eapp: "\<lbrakk>EApp e1 e2\<rbrakk> \<rho> = { v'. \<exists> f v. f \<in> \<lbrakk>e1\<rbrakk>\<rho> \<and> v \<in> \<lbrakk>e2\<rbrakk>\<rho> \<and> v' \<in> f \<bullet> v }" | 
   Eprim: "\<lbrakk>EPrim f e1 e2\<rbrakk> \<rho> = { v. \<exists> n1 n2. TNat n1 \<in> \<lbrakk>e1\<rbrakk>\<rho> 
